code/ecdsap256/Hacl.Impl.P256.MontgomeryMultiplication.fst
@@ -26,7 +26,7 @@ open Hacl.Spec.P256.MontgomeryMultiplication
 #set-options "--z3rlimit 100"
 
 inline_for_extraction noextract
-val add8_without_carry1: t: widefelem -> t1: widefelem -> result: widefelem  -> Stack unit
+val add8_without_carry1: t: widefelem P256 -> t1: widefelem P256 -> result: widefelem P256 -> Stack unit
   (requires fun h -> 
     live h t /\ live h t1 /\ live h result /\ eq_or_disjoint t1 result /\ 
     eq_or_disjoint t result /\ wide_as_nat h t1 < pow2 320 /\ wide_as_nat h t < prime256 * prime256
@@ -38,7 +38,7 @@ let add8_without_carry1 t t1 result  =
     assert_norm (pow2 320 + prime256 * prime256 < pow2 512)
 
 inline_for_extraction
-val montgomery_multiplication_round: t: widefelem -> round: widefelem -> Stack unit 
+val montgomery_multiplication_round: t: widefelem P256 -> round: widefelem P256 -> Stack unit 
   (requires fun h -> live h t /\ live h round /\ wide_as_nat h t < prime256 * prime256)
   (ensures fun h0 _ h1 -> modifies (loc round)  h0 h1 /\
     wide_as_nat h1 round = (wide_as_nat h0 t + prime256 * (wide_as_nat h0 t % pow2 64)) / pow2 64
@@ -73,7 +73,7 @@ let montgomery_multiplication_one_round_proof t result co =
 
 
 inline_for_extraction noextract
-val montgomery_multiplication_round_twice: t: widefelem -> result: widefelem -> Stack unit 
+val montgomery_multiplication_round_twice: t: widefelem P256 -> result: widefelem P256 -> Stack unit 
   (requires fun h -> live h t /\ live h result  /\ wide_as_nat h t < prime256 * prime256)
   (ensures fun h0 _ h1 -> 
     modifies (loc result) h0 h1 /\
@@ -92,20 +92,20 @@ let montgomery_multiplication_round_twice t result =
       let h0 = ST.get() in 
     montgomery_multiplication_round t tempRound; 
       let h1 = ST.get() in 
-      montgomery_multiplication_one_round_proof (wide_as_nat h0 t)  (wide_as_nat h1 tempRound) (wide_as_nat h0 t);
+      montgomery_multiplication_one_round_proof (wide_as_nat h0 t)  (wide_as_nat #P256 h1 tempRound) (wide_as_nat h0 t);
     montgomery_multiplication_round tempRound result;
       let h2 = ST.get() in 
-      montgomery_multiplication_one_round_proof (wide_as_nat h1 tempRound) (wide_as_nat h2 result) (wide_as_nat h0 t * modp_inv2_prime (pow2 64) prime256);
+      montgomery_multiplication_one_round_proof (wide_as_nat #P256 h1 tempRound) (wide_as_nat h2 result) (wide_as_nat h0 t * modp_inv2_prime (pow2 64) prime256);
       lemma_montgomery_mod_inverse_addition (wide_as_nat h0 t);
   pop_frame()
 
 
-val montgomery_multiplication_buffer_by_one: a: felem -> result: felem ->  Stack unit
-  (requires (fun h -> live h a /\ as_nat h a < prime256 /\ live h result)) 
+val montgomery_multiplication_buffer_by_one: a: felem P256 -> result: felem P256 -> Stack unit
+  (requires (fun h -> live h a /\ as_nat P256 h a < prime256 /\ live h result)) 
   (ensures (fun h0 _ h1 -> 
     modifies (loc result) h0 h1 /\ 
-    as_nat h1 result  = (as_nat h0 a * modp_inv2_prime (pow2 256) prime256) % prime256 /\
-    as_nat h1 result = fromDomain_ (as_nat h0 a))
+    as_nat P256 h1 result  = (as_nat P256 h0 a * modp_inv2_prime (pow2 256) prime256) % prime256 /\
+    as_nat P256 h1 result = fromDomain_ (as_nat P256 h0 a))
   )
 
 
@@ -120,38 +120,38 @@ let montgomery_multiplication_buffer_by_one a result =
       let h0 = ST.get() in 
     copy t_low a; 
       let h1 = ST.get() in 
-      assert(wide_as_nat h0 t = as_nat h0 t_low + as_nat h0 t_high * pow2 256);
+      assert(wide_as_nat #P256 h0 t = as_nat P256 h0 t_low + as_nat P256 h0 t_high * pow2 256);
       assert_norm (prime256 < prime256 * prime256);
     montgomery_multiplication_round_twice t round2;
       let h2 = ST.get() in 
     montgomery_multiplication_round_twice round2 round4; 
-      lemma_montgomery_mod_inverse_addition2 (wide_as_nat h1 t);
-      lemma_mod_mul_distr_l (wide_as_nat h2 round2) (modp_inv2_prime (pow2 128) prime256) prime256;
-      lemma_mod_mul_distr_l (wide_as_nat h1 t * modp_inv2_prime (pow2 128) prime256) (modp_inv2_prime (pow2 128) prime256) prime256;
-	mul_lemma_2 (wide_as_nat h1 t % pow2 64) (pow2 64 - 1) prime256;
-	mul_lemma_2 (let round = (wide_as_nat h1 t + prime256 * (wide_as_nat h1 t % pow2 64)) / pow2 64 in round % pow2 64) (pow2 64 - 1) prime256;
+      lemma_montgomery_mod_inverse_addition2 (wide_as_nat #P256 h1 t);
+      lemma_mod_mul_distr_l (wide_as_nat #P256 h2 round2) (modp_inv2_prime (pow2 128) prime256) prime256;
+      lemma_mod_mul_distr_l (wide_as_nat #P256 h1 t * modp_inv2_prime (pow2 128) prime256) (modp_inv2_prime (pow2 128) prime256) prime256;
+	mul_lemma_2 (wide_as_nat #P256 h1 t % pow2 64) (pow2 64 - 1) prime256;
+	mul_lemma_2 (let round = (wide_as_nat #P256 h1 t + prime256 * (wide_as_nat #P256 h1 t % pow2 64)) / pow2 64 in round % pow2 64) (pow2 64 - 1) prime256;
 	mul_lemma_2 (
-	  let round = (wide_as_nat h1 t + prime256 * (wide_as_nat h1 t % pow2 64)) / pow2 64 in  
+	  let round = (wide_as_nat #P256 h1 t + prime256 * (wide_as_nat #P256 h1 t % pow2 64)) / pow2 64 in  
 	  let round2 = (round + prime256 * (round % pow2 64)) / pow2 64 in 
 	  round2 % pow2 64) (pow2 64 - 1) prime256;
 	mul_lemma_2 (	
-	  let round = (wide_as_nat h1 t + prime256 * (wide_as_nat h1 t % pow2 64)) / pow2 64 in  
+	  let round = (wide_as_nat #P256 h1 t + prime256 * (wide_as_nat #P256 h1 t % pow2 64)) / pow2 64 in  
 	  let round2 = (round + prime256 * (round % pow2 64)) / pow2 64 in 
 	  let round3 = (round2 + prime256 * (round2 % pow2 64)) / pow2 64 in   
 	  round3 % pow2 64) (pow2 64 - 1) prime256;
     reduction_prime256_2prime256_8_with_carry_impl round4 result;
-    lemmaFromDomain (as_nat h0 a);
+    lemmaFromDomain (as_nat P256 h0 a);
   pop_frame()  
 
 
-val montgomery_multiplication_buffer: a: felem -> b: felem -> result: felem ->  Stack unit
-  (requires (fun h -> live h a /\ as_nat h a < prime256 /\ live h b /\ live h result /\ as_nat h b < prime256)) 
+val montgomery_multiplication_buffer: a: felem P256 -> b: felem P256 -> result: felem P256 ->  Stack unit
+  (requires (fun h -> live h a /\ as_nat P256 h a < prime256 /\ live h b /\ live h result /\ as_nat P256 h b < prime256)) 
   (ensures (fun h0 _ h1 -> 
     modifies (loc result) h0 h1 /\  
-    as_nat h1 result < prime256 /\
-    as_nat h1 result = (as_nat h0 a * as_nat h0 b * modp_inv2_prime (pow2 256) prime256) % prime256 /\
-    as_nat h1 result = toDomain_ (fromDomain_ (as_nat h0 a) * fromDomain_ (as_nat h0 b) % prime256) /\
-    as_nat h1 result = toDomain_ (fromDomain_ (as_nat h0 a) * fromDomain_ (as_nat h0 b)))
+    as_nat P256 h1 result < prime256 /\
+    as_nat P256 h1 result = (as_nat P256 h0 a * as_nat P256 h0 b * modp_inv2_prime (pow2 256) prime256) % prime256 /\
+    as_nat P256 h1 result = toDomain_ (fromDomain_ (as_nat P256 h0 a) * fromDomain_ (as_nat P256 h0 b) % prime256) /\
+    as_nat P256 h1 result = toDomain_ (fromDomain_ (as_nat P256 h0 a) * fromDomain_ (as_nat P256 h0 b)))
   )
 
 
@@ -164,45 +164,45 @@ let montgomery_multiplication_buffer a b result =
       let h0 = ST.get() in 
     mul a b t;  
       let h1 = ST.get() in 
-      mul_lemma_ (as_nat h0 a) (as_nat h0 b) prime256;
+      mul_lemma_ (as_nat P256 h0 a) (as_nat P256 h0 b) prime256;
   montgomery_multiplication_round_twice t round2;
       let h2 = ST.get() in 
   montgomery_multiplication_round_twice round2 round4; 
       let h3 = ST.get() in 
-	lemma_montgomery_mod_inverse_addition2 (wide_as_nat h1 t);
-	lemma_mod_mul_distr_l (wide_as_nat h2 round2) (modp_inv2_prime (pow2 128) prime256) prime256;
-	lemma_mod_mul_distr_l (wide_as_nat h1 t * modp_inv2_prime (pow2 128) prime256) (modp_inv2_prime (pow2 128) prime256) prime256;
-      mul_lemma_2 (wide_as_nat h1 t % pow2 64) (pow2 64 - 1) prime256;
-      mul_lemma_ (as_nat h0 a) (as_nat h0 b) prime256;
+	lemma_montgomery_mod_inverse_addition2 (wide_as_nat #P256 h1 t);
+	lemma_mod_mul_distr_l (wide_as_nat #P256 h2 round2) (modp_inv2_prime (pow2 128) prime256) prime256;
+	lemma_mod_mul_distr_l (wide_as_nat #P256 h1 t * modp_inv2_prime (pow2 128) prime256) (modp_inv2_prime (pow2 128) prime256) prime256;
+      mul_lemma_2 (wide_as_nat #P256 h1 t % pow2 64) (pow2 64 - 1) prime256;
+      mul_lemma_ (as_nat P256 h0 a) (as_nat P256 h0 b) prime256;
       mul_lemma_1 ( 
-         let round = (wide_as_nat h1 t + prime256 * (wide_as_nat h1 t % pow2 64)) / pow2 64 in  
+         let round = (wide_as_nat #P256 h1 t + prime256 * (wide_as_nat #P256 h1 t % pow2 64)) / pow2 64 in  
 	 round % pow2 64) (pow2 64) prime256; 
       mul_lemma_1 ( 
-	let round = (wide_as_nat h1 t + prime256 * (wide_as_nat h1 t % pow2 64)) / pow2 64 in 
+	let round = (wide_as_nat #P256 h1 t + prime256 * (wide_as_nat #P256 h1 t % pow2 64)) / pow2 64 in 
 	let round2 = (round + prime256 * (round % pow2 64)) / pow2 64 in 
 	round2 % pow2 64) (pow2 64) prime256; 
       mul_lemma_1 ( 
-	let round = (wide_as_nat h1 t + prime256 * (wide_as_nat h1 t % pow2 64)) / pow2 64 in 
+	let round = (wide_as_nat #P256 h1 t + prime256 * (wide_as_nat #P256 h1 t % pow2 64)) / pow2 64 in 
 	let round2 = (round + prime256 * (round % pow2 64)) / pow2 64 in 
 	let round3 = (round2 + prime256 * (round2 % pow2 64)) / pow2 64 in 
 	round3 % pow2 64) (pow2 64) prime256;  
       assert_norm((prime256 * pow2 64 + (prime256 * pow2 64 + (prime256 * pow2 64 + ((pow2 64 - 1) * prime256 + prime256 * prime256) / pow2 64) / pow2 64)/ pow2 64) / pow2 64 < 2 * prime256);
   reduction_prime256_2prime256_8_with_carry_impl round4 result; 
-  lemmaFromDomainToDomain (as_nat h0 a);
-  lemmaFromDomainToDomain (as_nat h0 b);
-  multiplicationInDomainNat #(fromDomain_ (as_nat h0 a)) #(fromDomain_ (as_nat h0 b))  (as_nat h0 a) (as_nat h0 b);
-  inDomain_mod_is_not_mod (fromDomain_ (as_nat h0 a) * fromDomain_ (as_nat h0 b));
+  lemmaFromDomainToDomain (as_nat P256 h0 a);
+  lemmaFromDomainToDomain (as_nat P256 h0 b);
+  multiplicationInDomainNat #(fromDomain_ (as_nat P256 h0 a)) #(fromDomain_ (as_nat P256 h0 b))  (as_nat P256 h0 a) (as_nat P256 h0 b);
+  inDomain_mod_is_not_mod (fromDomain_ (as_nat P256 h0 a) * fromDomain_ (as_nat P256 h0 b));
   pop_frame()  
 
 
-val montgomery_square_buffer: a: felem -> result: felem ->  Stack unit
-  (requires (fun h -> live h a /\ as_nat h a < prime256 /\ live h result)) 
+val montgomery_square_buffer: a: felem P256 -> result: felem P256 ->  Stack unit
+  (requires (fun h -> live h a /\ as_nat P256 h a < prime256 /\ live h result)) 
   (ensures (fun h0 _ h1 -> 
     modifies (loc result) h0 h1 /\  
-    as_nat h1 result < prime256 /\ 
-    as_nat h1 result = (as_nat h0 a * as_nat h0 a * modp_inv2_prime (pow2 256) prime256) % prime256 /\
-    as_nat h1 result = toDomain_ (fromDomain_ (as_nat h0 a) * fromDomain_ (as_nat h0 a) % prime256) /\
-    as_nat h1 result = toDomain_ (fromDomain_ (as_nat h0 a) * fromDomain_ (as_nat h0 a)))
+    as_nat P256 h1 result < prime256 /\ 
+    as_nat P256 h1 result = (as_nat P256 h0 a * as_nat P256 h0 a * modp_inv2_prime (pow2 256) prime256) % prime256 /\
+    as_nat P256 h1 result = toDomain_ (fromDomain_ (as_nat P256 h0 a) * fromDomain_ (as_nat P256 h0 a) % prime256) /\
+    as_nat P256 h1 result = toDomain_ (fromDomain_ (as_nat P256 h0 a) * fromDomain_ (as_nat P256 h0 a)))
   )
 
 
@@ -215,60 +215,60 @@ let montgomery_square_buffer a result =
       let h0 = ST.get() in 
     sq a t;  
       let h1 = ST.get() in 
-      mul_lemma_ (as_nat h0 a) (as_nat h0 a) prime256;
+      mul_lemma_ (as_nat P256 h0 a) (as_nat P256 h0 a) prime256;
   montgomery_multiplication_round_twice t round2;
       let h2 = ST.get() in 
   montgomery_multiplication_round_twice round2 round4; 
       let h3 = ST.get() in 
-  lemma_montgomery_mod_inverse_addition2 (wide_as_nat h1 t);
-  lemma_mod_mul_distr_l (wide_as_nat h2 round2) (modp_inv2_prime (pow2 128) prime256) prime256;
-  lemma_mod_mul_distr_l (wide_as_nat h1 t * modp_inv2_prime (pow2 128) prime256) (modp_inv2_prime (pow2 128) prime256) prime256;
-      mul_lemma_2 (wide_as_nat h1 t % pow2 64) (pow2 64 - 1) prime256;
-      mul_lemma_ (as_nat h0 a) (as_nat h0 a) prime256;
+  lemma_montgomery_mod_inverse_addition2 (wide_as_nat #P256 h1 t);
+  lemma_mod_mul_distr_l (wide_as_nat #P256 h2 round2) (modp_inv2_prime (pow2 128) prime256) prime256;
+  lemma_mod_mul_distr_l (wide_as_nat #P256 h1 t * modp_inv2_prime (pow2 128) prime256) (modp_inv2_prime (pow2 128) prime256) prime256;
+      mul_lemma_2 (wide_as_nat #P256 h1 t % pow2 64) (pow2 64 - 1) prime256;
+      mul_lemma_ (as_nat P256 h0 a) (as_nat P256 h0 a) prime256;
       mul_lemma_1 ( 
-         let round = (wide_as_nat h1 t + prime256 * (wide_as_nat h1 t % pow2 64)) / pow2 64 in  
+         let round = (wide_as_nat #P256 h1 t + prime256 * (wide_as_nat #P256 h1 t % pow2 64)) / pow2 64 in  
    round % pow2 64) (pow2 64) prime256; 
       mul_lemma_1 ( 
-  let round = (wide_as_nat h1 t + prime256 * (wide_as_nat h1 t % pow2 64)) / pow2 64 in 
+  let round = (wide_as_nat #P256  h1 t + prime256 * (wide_as_nat #P256 h1 t % pow2 64)) / pow2 64 in 
   let round2 = (round + prime256 * (round % pow2 64)) / pow2 64 in 
   round2 % pow2 64) (pow2 64) prime256; 
       mul_lemma_1 ( 
-  let round = (wide_as_nat h1 t + prime256 * (wide_as_nat h1 t % pow2 64)) / pow2 64 in 
+  let round = (wide_as_nat #P256 h1 t + prime256 * (wide_as_nat #P256 h1 t % pow2 64)) / pow2 64 in 
   let round2 = (round + prime256 * (round % pow2 64)) / pow2 64 in 
   let round3 = (round2 + prime256 * (round2 % pow2 64)) / pow2 64 in 
   round3 % pow2 64) (pow2 64) prime256;  
       assert_norm((prime256 * pow2 64 + (prime256 * pow2 64 + (prime256 * pow2 64 + ((pow2 64 - 1) * prime256 + prime256 * prime256) / pow2 64) / pow2 64)/ pow2 64) / pow2 64 < 2 * prime256);
   reduction_prime256_2prime256_8_with_carry_impl round4 result; 
-  lemmaFromDomainToDomain (as_nat h0 a);
-  multiplicationInDomainNat #(fromDomain_ (as_nat h0 a)) #(fromDomain_ (as_nat h0 a))  (as_nat h0 a) (as_nat h0 a);
-  inDomain_mod_is_not_mod (fromDomain_ (as_nat h0 a) * fromDomain_ (as_nat h0 a));
+  lemmaFromDomainToDomain (as_nat P256 h0 a);
+  multiplicationInDomainNat #(fromDomain_ (as_nat P256 h0 a)) #(fromDomain_ (as_nat P256 h0 a))  (as_nat P256 h0 a) (as_nat P256 h0 a);
+  inDomain_mod_is_not_mod (fromDomain_ (as_nat P256 h0 a) * fromDomain_ (as_nat P256 h0 a));
   pop_frame()  
 
 
 #reset-options "--z3rlimit 500" 
 
-val fsquarePowN: n: size_t -> a: felem -> Stack unit 
-  (requires (fun h -> live h a /\ as_nat h a < prime256)) 
+val fsquarePowN: n: size_t -> a: felem P256 -> Stack unit 
+  (requires (fun h -> live h a /\ as_nat P256 h a < prime256)) 
   (ensures (fun h0 _ h1 -> 
-    modifies (loc a) h0 h1 /\  as_nat h1 a < prime256 /\ 
-    (let k = fromDomain_(as_nat h0 a) in as_nat h1 a = toDomain_ (pow k (pow2 (v n)))))
+    modifies (loc a) h0 h1 /\  as_nat P256 h1 a < prime256 /\ 
+    (let k = fromDomain_(as_nat P256 h0 a) in as_nat P256 h1 a = toDomain_ (pow k (pow2 (v n)))))
   )
 
 let fsquarePowN n a = 
   let h0 = ST.get() in  
-  lemmaFromDomainToDomain (as_nat h0 a); 
+  lemmaFromDomainToDomain (as_nat P256 h0 a); 
   assert_norm (pow2 0 == 1); 
   let inv (h0: HyperStack.mem) (h1: HyperStack.mem) (i: nat) : Type0 =
-    let k = fromDomain_ (as_nat h0 a) in 
-    as_nat h1 a = toDomain_ (pow k (pow2 i)) /\
-    as_nat h1 a < prime256 /\ live h1 a /\ modifies1 a h0 h1  in 
-  power_one (fromDomain_ (as_nat h0 a)); 
+    let k = fromDomain_ (as_nat P256 h0 a) in 
+    as_nat P256 h1 a = toDomain_ (pow k (pow2 i)) /\
+    as_nat P256 h1 a < prime256 /\ live h1 a /\ modifies1 a h0 h1  in 
+  power_one (fromDomain_ (as_nat P256 h0 a)); 
   for (size 0) n (inv h0) (fun x -> 
     let h0_ = ST.get() in 
      montgomery_square_buffer a a; 
-     let k = fromDomain_ (as_nat h0 a) in  
-     inDomain_mod_is_not_mod (fromDomain_ (as_nat h0_ a) * fromDomain_ (as_nat h0_ a)); 
-     lemmaFromDomainToDomainModuloPrime (let k = fromDomain_ (as_nat h0 a) in pow k (pow2 (v x)));
+     let k = fromDomain_ (as_nat P256 h0 a) in  
+     inDomain_mod_is_not_mod (fromDomain_ (as_nat P256 h0_ a) * fromDomain_ (as_nat P256 h0_ a)); 
+     lemmaFromDomainToDomainModuloPrime (let k = fromDomain_ (as_nat P256 h0 a) in pow k (pow2 (v x)));
      modulo_distributivity_mult (pow k (pow2 (v x))) (pow k (pow2 (v x))) prime256; 
      pow_plus k  (pow2 (v x)) (pow2 (v x )); 
      pow2_double_sum (v x);
@@ -276,14 +276,14 @@ let fsquarePowN n a =
   )
 
 
-val fsquarePowNminusOne: n: size_t -> a: felem -> tempBuffer: felem -> Stack unit 
-  (requires (fun h -> live h a /\ live h tempBuffer /\ as_nat h a < prime256 /\ disjoint a tempBuffer)) 
+val fsquarePowNminusOne: n: size_t -> a: felem P256 -> tempBuffer: felem P256 -> Stack unit 
+  (requires (fun h -> live h a /\ live h tempBuffer /\ as_nat P256 h a < prime256 /\ disjoint a tempBuffer)) 
   (ensures (fun h0 _ h1 -> 
-    as_nat h1 a < prime256 /\ as_nat h1 tempBuffer < prime256 /\ 
+    as_nat P256 h1 a < prime256 /\ as_nat P256 h1 tempBuffer < prime256 /\ 
     modifies (loc a |+| loc tempBuffer) h0 h1 /\ 
     (
-      let k = fromDomain_ (as_nat h0 a) in  
-      as_nat h1 a = toDomain_ (pow k (pow2 (v n))) /\ as_nat h1 tempBuffer = toDomain_ (pow k (pow2 (v n) -1 )))
+      let k = fromDomain_ (as_nat P256 h0 a) in  
+      as_nat P256 h1 a = toDomain_ (pow k (pow2 (v n))) /\ as_nat P256 h1 tempBuffer = toDomain_ (pow k (pow2 (v n) -1 )))
     )
    )
 
@@ -296,25 +296,25 @@ let fsquarePowNminusOne n a b =
   Lib.Buffer.upd b (size 3) (u64 4294967294);
 
   let one = (u64 1, u64 18446744069414584320, u64 18446744073709551615, u64 4294967294) in 
-      lemmaFromDomainToDomain (as_nat h0 a);
+      lemmaFromDomainToDomain (as_nat P256 h0 a);
       lemmaToDomain 1;
       assert_norm (1 + pow2 64 * 18446744069414584320 + pow2 64 * pow2 64 * 18446744073709551615 + pow2 64 * pow2 64 * pow2 64 * 4294967294 = 26959946660873538059280334323183841250350249843923952699046031785985);
       assert_norm (pow2 256 % prime256 == 26959946660873538059280334323183841250350249843923952699046031785985);
       assert_norm (as_nat4 one = toDomain_(1));
 
   let inv (h0: HyperStack.mem) (h1: HyperStack.mem) (i: nat) : Type0 = 
-    let k = fromDomain_(as_nat h0 a) in 
-    as_nat h1 b = toDomain_ (pow k (pow2 i - 1)) /\ as_nat h1 a < prime256 /\ live h1 a /\
-    as_nat h1 a = toDomain_ (pow k (pow2 i)) /\ as_nat h1 b < prime256 /\ live h1 b /\ modifies (loc a |+| loc b) h0 h1 in 
+    let k = fromDomain_(as_nat P256 h0 a) in 
+    as_nat P256 h1 b = toDomain_ (pow k (pow2 i - 1)) /\ as_nat  P256 h1 a < prime256 /\ live h1 a /\
+    as_nat P256 h1 a = toDomain_ (pow k (pow2 i)) /\ as_nat P256 h1 b < prime256 /\ live h1 b /\ modifies (loc a |+| loc b) h0 h1 in 
   for (size 0) n (inv h0) (fun x -> 
     let h0_ = ST.get() in 
     montgomery_multiplication_buffer b a b;
     montgomery_square_buffer a a;
-    let k = fromDomain_ (as_nat h0 a) in 
-    inDomain_mod_is_not_mod (fromDomain_ (as_nat h0_ b) * fromDomain_ (as_nat h0_ a));
-    inDomain_mod_is_not_mod (fromDomain_ (as_nat h0_ a) * fromDomain_ (as_nat h0_ a));
+    let k = fromDomain_ (as_nat P256 h0 a) in 
+    inDomain_mod_is_not_mod (fromDomain_ (as_nat P256 h0_ b) * fromDomain_ (as_nat P256 h0_ a));
+    inDomain_mod_is_not_mod (fromDomain_ (as_nat P256 h0_ a) * fromDomain_ (as_nat P256 h0_ a));
 
-    lemmaFromDomainToDomainModuloPrime (pow k (pow2 (v x) -1 ));
+    lemmaFromDomainToDomainModuloPrime (pow k (pow2 (v x) - 1));
     lemmaFromDomainToDomainModuloPrime (pow k (pow2 (v x)));
     modulo_distributivity_mult (pow k (pow2 (v x) - 1)) (pow k (pow2 (v x))) prime256;
     modulo_distributivity_mult (pow k (pow2 (v x))) (pow k (pow2 (v x))) prime256;
@@ -329,10 +329,10 @@ let fsquarePowNminusOne n a b =
 
 
 inline_for_extraction noextract   
-val norm_part_one: a: felem -> tempBuffer: lbuffer uint64 (size 8) -> 
-  Stack unit (requires fun h -> live h a /\ live h tempBuffer /\ disjoint a tempBuffer /\  as_nat h a < prime256)
-  (ensures fun h0 _ h1 -> modifies1 tempBuffer h0 h1 /\ (let buffer_result = gsub tempBuffer (size 4) (size 4) in as_nat h1 buffer_result < prime256 /\ 
-  (let k = fromDomain_ (as_nat h0 a) in as_nat h1 buffer_result = toDomain_(pow k ((pow2 32 - 1) * pow2 224) % prime256))))
+val norm_part_one: a: felem P256 -> tempBuffer: lbuffer uint64 (size 8) -> 
+  Stack unit (requires fun h -> live h a /\ live h tempBuffer /\ disjoint a tempBuffer /\  as_nat P256 h a < prime256)
+  (ensures fun h0 _ h1 -> modifies1 tempBuffer h0 h1 /\ (let buffer_result = gsub tempBuffer (size 4) (size 4) in as_nat P256 h1 buffer_result < prime256 /\ 
+  (let k = fromDomain_ (as_nat P256 h0 a) in as_nat P256 h1 buffer_result = toDomain_(pow k ((pow2 32 - 1) * pow2 224) % prime256))))
     
 let norm_part_one a tempBuffer = 
     let h0 = ST.get() in 
@@ -344,7 +344,7 @@ let norm_part_one a tempBuffer =
   fsquarePowNminusOne (size 32) buffer_a buffer_b;
   fsquarePowN (size 224) buffer_b;
 
-  let k = fromDomain_ (as_nat h0 a) in 
+  let k = fromDomain_ (as_nat P256 h0 a) in 
   lemmaFromDomainToDomainModuloPrime (pow k (pow2 32 - 1));
   let k_powers = pow k (pow2 32 - 1) in 
   let k_prime = k_powers % prime256 in 
@@ -354,24 +354,24 @@ let norm_part_one a tempBuffer =
  
  
 inline_for_extraction noextract   
-val norm_part_two: a: felem -> tempBuffer: lbuffer uint64 (size 4) -> 
-  Stack unit (requires fun h -> live h a /\ live h tempBuffer /\ disjoint a tempBuffer /\  as_nat h a < prime256)
-  (ensures fun h0 _ h1 -> as_nat h1 tempBuffer < prime256 /\ modifies1 tempBuffer h0 h1 /\
-    (let k = fromDomain_ (as_nat h0 a) in as_nat h1 tempBuffer = toDomain_(pow k (pow2 192) % prime256)))
+val norm_part_two: a: felem P256 -> tempBuffer: lbuffer uint64 (size 4) -> 
+  Stack unit (requires fun h -> live h a /\ live h tempBuffer /\ disjoint a tempBuffer /\  as_nat P256 h a < prime256)
+  (ensures fun h0 _ h1 -> as_nat P256 h1 tempBuffer < prime256 /\ modifies1 tempBuffer h0 h1 /\
+    (let k = fromDomain_ (as_nat P256 h0 a) in as_nat P256 h1 tempBuffer = toDomain_(pow k (pow2 192) % prime256)))
     
 let norm_part_two a tempBuffer = 
   let h0 = ST.get() in 
   Lib.Buffer.copy tempBuffer a;
   fsquarePowN (size 192) tempBuffer;
-  let k = fromDomain_ (as_nat h0 a) in 
+  let k = fromDomain_ (as_nat P256 h0 a) in 
   inDomain_mod_is_not_mod (pow k (pow2 192))
 
 inline_for_extraction noextract   
-val norm_part_three:a: felem -> tempBuffer: lbuffer uint64 (size 8) -> 
+val norm_part_three:a: felem P256 -> tempBuffer: lbuffer uint64 (size 8) -> 
   Stack unit (requires fun h -> live h a /\ live h tempBuffer /\ disjoint a tempBuffer /\  
-   as_nat h a < prime256)   
-  (ensures fun h0 _ h1 ->  modifies1 tempBuffer h0 h1 /\ (let buffer_result = gsub tempBuffer (size 4) (size 4) in as_nat h1 buffer_result < prime256
-    /\ (let k = fromDomain_ (as_nat h0 a) in as_nat h1 buffer_result = toDomain_(pow k ((pow2 94 - 1) * pow2 2) % prime256))))
+   as_nat P256 h a < prime256)   
+  (ensures fun h0 _ h1 ->  modifies1 tempBuffer h0 h1 /\ (let buffer_result = gsub tempBuffer (size 4) (size 4) in as_nat P256 h1 buffer_result < prime256
+    /\ (let k = fromDomain_ (as_nat P256 h0 a) in as_nat P256 h1 buffer_result = toDomain_(pow k ((pow2 94 - 1) * pow2 2) % prime256))))
 
 let norm_part_three a tempBuffer = 
   let h0 = ST.get() in 
@@ -383,7 +383,7 @@ let norm_part_three a tempBuffer =
   fsquarePowNminusOne (size 94) buffer_a buffer_b;
   fsquarePowN (size 2) buffer_b;
 
-  let k = fromDomain_ (as_nat h0 a) in 
+  let k = fromDomain_ (as_nat P256 h0 a) in 
   lemmaFromDomainToDomainModuloPrime (pow k (pow2 94 - 1));
   let k_powers = pow k (pow2 94 - 1) in 
   let k_prime = k_powers % prime256 in 
@@ -416,11 +416,11 @@ val lemma_mul_nat: a: nat -> b: nat -> Lemma (a * b >= 0)
 let lemma_mul_nat a b = ()
 
 
-val exponent: a: felem ->result: felem -> tempBuffer: lbuffer uint64 (size 20) ->  Stack unit
+val exponent: a: felem P256 -> result: felem P256 -> tempBuffer: lbuffer uint64 (size 20) ->  Stack unit
   (requires fun h -> live h a /\ live h tempBuffer /\ live h result /\ disjoint tempBuffer result /\ 
-  disjoint a tempBuffer /\ as_nat h a < prime256)
-  (ensures fun h0 _ h1 -> modifies2 result tempBuffer h0 h1 /\ (let k = fromDomain_ (as_nat h0 a) in 
-    as_nat h1 result =  toDomain_ ((pow k (prime256-2)) % prime256)))
+  disjoint a tempBuffer /\ as_nat P256 h a < prime256)
+  (ensures fun h0 _ h1 -> modifies2 result tempBuffer h0 h1 /\ (let k = fromDomain_ (as_nat P256 h0 a) in 
+    as_nat P256 h1 result =  toDomain_ ((pow k (prime256-2)) % prime256)))
 
 
 #reset-options " --z3rlimit 200"
@@ -450,7 +450,7 @@ let exponent a result tempBuffer =
   assert_norm ((pow2 94 - 1) * pow2 2 >= 0);
 
   
-  let k = fromDomain_ (as_nat h0 a) in 
+  let k = fromDomain_ (as_nat P256 h0 a) in 
   let power1 = pow k ((pow2 32 - 1) * pow2 224) in 
   let power2 = pow k (pow2 192) in 
   let power3 = pow k ((pow2 94 - 1) * pow2 2) in 
